WIP tutorial

demos/tutorial.v
@@ -22,6 +22,181 @@
 ========
 Tutorial
 ========
+
+Welcome! This is a quick primer for designing circuits with Cava. We'll walk
+through a few small examples end-to-end.
+
+.. coq:: none
 |*)
 
-Check nat.
+Require Import ExtLib.Structures.Monads.
+Import MonadNotation.
+Open Scope monad_scope.
+
+Require Import Cava.Acorn.Acorn.
+
+(*|
+Example 1 : Inverter
+====================
+
+To start, let's define a 1-bit inverter.
+|*)
+
+Definition inverter
+           {signal : SignalType -> Type}
+           {semantics : Cava signal}
+  : Circuit (signal Bit) (signal Bit) :=
+  Comb inv.
+
+(*|
+A few things to notice here:
+
+* ``SignalType`` is Cava's type system. The inverter is parameterized over
+  ``signal``, which converts ``SignalType``\ s to Coq types. ``Bit`` is one
+  example of a ``SignalType``; we'll see more examples later on.
+* ``Comb`` is short for "combinational"; our inverter has no loops, registers,
+  or timing requirements, so it is a purely combinational circuit.
+* The inverter is also paramterized over ``semantics``, an instance of the
+  typeclass ``Cava``. This instance provides implementations of circuit
+  primitives, such as 1-bit logic gates. One primitive is a 1-bit inverter
+  ``inv``, so our inverter is just a simple invocation of the primitive.
+
+Normally, we'd write circuit definitions a little more concisely by writing them
+inside a ``Section`` that contains ``signal`` and ``semantics`` as context
+variables, like this:
+|*)
+
+Section WithCava.
+  Context {signal} {semantics : Cava signal}.
+
+  Definition inverter_concise : Circuit (signal Bit) (signal Bit)
+    := Comb inv.
+
+(*|
+For the rest of the circuit definitions in this tutorial, you can assume that
+we're inside the section and that every definition is parameterized over the
+``signal`` and ``semantics`` context variables.
+
+Back to our inverter. Let's take a closer look at the ``inv`` primitive.
+|*)
+
+  About inv.
+
+(*|
+You can see in the type signature ``signal Bit -> cava (signal Bit)`` that
+``inv`` is defined as a pure Coq function in terms of a monad called
+``cava``. The ``cava`` monad, like ``inv``, is provided by ``semantics``. The
+monad is used to preserve sharing; it's semantically different in Cava to write::
+
+  x <- inv zero ;;
+  y <- inv zero ;;
+  xor2 x y
+
+than it is to write::
+
+  x <- inv zero ;;
+  xor2 x x
+
+Both expressions have the same meaning, and if we were using Gallina ``let``
+binders there would be no difference. But the generated circuit will use two
+wires for the first definition, and fork the same wire in the second. As circuit
+diagrams, this is the difference between::
+
+         +-----+      +-----+
+  1 ---- | inv |------|     |
+         +-----+      | xor | ---- out
+         +-----+      |     |
+  1 ---- | inv | ---- |     |
+         +-----+      +-----+
+
+and::
+
+                            +-----+
+                     +----- |     |
+                     |      | xor | ---- out
+         +-----+     |      |     |
+  1 ---- | inv | ----+----- |     |
+         +-----+            +-----+
+
+This difference isn't significant in determining what the value of ``out`` will
+be, but it can be very useful when trying to exercise fine-grained control over
+circuit layout and area!
+
+Parameterizing over the ``cava`` monad and primitive implementations allows us
+to use different instances of ``Cava`` to interpret the same circuit definition
+in different ways. For instance, one ``Cava`` instance creates a netlist from
+the circuit definition by using a state monad that adds and connects wires in
+the background. Defining a purely combinational circuit is simply defining a
+Gallina function in terms of the ``cava`` monad and ``SignalType``.
+
+.. coq:: none
+|*)
+
+  Definition test1 : cava (signal Bit) :=
+    x <- inv one ;;
+    xor2 (x, x).
+  Definition test2 : cava (signal Bit) :=
+    x <- inv one ;;
+    y <- inv one ;;
+    xor2 (x, y).
+End WithCava.
+
+Require Import Coq.Strings.String.
+Require Import Coq.Lists.List.
+Import ListNotations.
+Require Import Cava.Cava.
+
+Definition test_interface
+  := sequentialInterface "test_interface"
+     "clk" PositiveEdge "rst" PositiveEdge
+     [mkPort "i" Void]
+     [mkPort "o" Bit]
+     [].
+
+(* does Circuit need an input type? or can it have just one type with function applications? *)
+
+
+Require Import Coq.NArith.NArith.
+
+Compute (makeCircuitNetlist test_interface (Comb (fun _ => test1))).
+(*      = {| *)
+(*   netNumber := 2; *)
+(*   vectorNumber := 0; *)
+(*   vectorDeclarations := []; *)
+(*   externalDeclarations := []; *)
+(*   clockNet := Some (NamedWire "clk"); *)
+(*   clockEdge := PositiveEdge; *)
+(*   resetNet := Some (NamedWire "rst"); *)
+(*   resetEdge := PositiveEdge; *)
+(*   module := {| *)
+(*             moduleName := "test_interface"; *)
+(*             netlist := [AssignSignal (NamedWire "o") (Wire 1); *)
+(*                        Xor (Wire 0) (Wire 0) (Wire 1);  *)
+(*                        Not Vcc (Wire 0)]; *)
+(*             inputs := [{| port_name := "rst"; port_type := Bit |}; *)
+(*                       {| port_name := "clk"; port_type := Bit |}]; *)
+(*             outputs := [{| port_name := "o"; port_type := Bit |}] |}; *)
+(*   libraryModules := [] |} *)
+(* : CavaState *)
+
+
+Compute (makeCircuitNetlist test_interface (Comb (fun _ => test2))).
+(* = {| *)
+(*   netNumber := 3; *)
+(*   vectorNumber := 0; *)
+(*   vectorDeclarations := []; *)
+(*   externalDeclarations := []; *)
+(*   clockNet := Some (NamedWire "clk"); *)
+(*   clockEdge := PositiveEdge; *)
+(*   resetNet := Some (NamedWire "rst"); *)
+(*   resetEdge := PositiveEdge; *)
+(*   module := {| *)
+(*             moduleName := "test_interface"; *)
+(*             netlist := [AssignSignal (NamedWire "o") (Wire 2); *)
+(*                        Xor (Wire 0) (Wire 1) (Wire 2);  *)
+(*                        Not Vcc (Wire 1); Not Vcc (Wire 0)]; *)
+(*             inputs := [{| port_name := "rst"; port_type := Bit |}; *)
+(*                       {| port_name := "clk"; port_type := Bit |}]; *)
+(*             outputs := [{| port_name := "o"; port_type := Bit |}] |}; *)
+(*   libraryModules := [] |} *)
+(* : CavaState *)
